# $f(n)$
$$f(n) = 2n$$

# $g(n)$
$$ g(n)=\begin{cases}
    0 & \text{if } n=0\\
    2 & \text{if } n=1 \\
    f(g(n-1)) & \text{o.w.}
\end{cases}$$
Since we know that $f(n) = 2n$, it becomes
$$ g(n)=\begin{cases}
    0 & \text{if } n=0\\
    2 & \text{if } n=1 \\
    2 g(n-1) & \text{o.w.}
\end{cases}$$
This recursive definition can be reduced to
$$ g(n)=\begin{cases}
    0 & \text{if } n=0\\
    2 & \text{if } n=1 \\
    2^n & \text{o.w.}
\end{cases}$$
And finally,
$$ g(n)=\begin{cases}
    0 & \text{if } n=0\\
    2^n & \text{o.w.}
\end{cases}$$


# $h(n)$
$$ h(n) = \begin{cases}
    0 & \text{if } n = 0 \\
    2 & \text{if } n = 1 \\
    g(h(n-1)) & \text{o.w.}
\end{cases}$$
Since we figured out about $g$, we know that
$$ h(n) = \begin{cases}
    0 & \text{if } n = 0 \\
    2 & \text{if } n = 1 \\
    2^{h(n-1)} & \text{o.w.}
\end{cases}$$
This recursive definition can be reduced to
$$ h(n) = \begin{cases}
    0 & \text{if } n = 0 \\
    2 & \text{if } n = 1 \\
    2^{2^{...^{2}}} & \text{o.w. where the number of 2's appear is } n
\end{cases}$$
And finally,
$$ h(n) = \begin{cases}
    0 & \text{if } n = 0 \\
    2^{2^{...^{2}}} & \text{o.w. where the number of 2's appear is } n
\end{cases}$$