# Before we start, about $\varphi$ and $\psi$
We will use the fact that both $\varphi$ and $\psi$ are the roots of the equation
$$x^2 - x - 1 = 0 $$

# Indunction
## Formula we want to prove
$$
Fib(n) = {\varphi^n - \psi^n\over\sqrt5}
$$
## Base case 1 : $n = 0$
$$
\begin{split}
Fib(0) & = {\varphi^0 - \psi^0\over\sqrt5}\\
& = {1-1\over\sqrt5}\\
& = 0
\end{split}
$$
## Base case 2 : $n = 1$
$$
\begin{split}
Fib(1) & = {\varphi^1 - \psi^1\over\sqrt5}\\
& = {\sqrt5\over\sqrt5}\\
& = 1
\end{split}
$$
## Induction Step
We're gonna prove that when the formula holds for $k <=n$, it also holds on $n+1$
$$
\begin{split}
Fib(n+1) & = Fib(n) + Fib(n-1)\\
& = {\varphi^{n} - \psi^{n}\over\sqrt5} + {\varphi^{n-1} - \psi^{n-1}\over\sqrt5}\\
& = {\varphi^{n-1}(\varphi + 1) - \psi^{n-1}(\psi + 1)\over\sqrt5}\\
& = {\varphi^{n+1} - \psi^{n+1}\over\sqrt5}\\
\end{split}
$$
First line comes from the definition of $Fib$.   
Second line comes from the fact it hold for all $k <= n$.   
Fourth line comes from the fact we checked before we started about $\varphi$ and $\psi$.